Měl by ji nosit v pravé ruce (za předpokladu, že nosit, znamená se o ni opírat)

![plan](F:\Docs\CTU\b201\Biomechanics\8\plan.png)
$$
|\vec{F_A}| = |\vec{F_B}|\\
d = a+b+c\\
\vec{r_W} [ -b; 0 ]\\
\vec{r_S} [ a; 0 ]\\
\vec{r_A} [ a+c; 0 ]\\
\vec{r_B} [ -(b+d); 0 ]\\
\vec{W} [0, -W]; W=(W_B-W_R)\\
\vec{F_S} [F_S\cos{\gamma}; -F_S\sin{\gamma}]\\
\vec{F_A} [0, F_A]\\
\vec{F_A} [0, F_B]\\
$$

### Pro A

$$
\begin{align}
\sum{F_{ix}} = 0 &\Rightarrow F_S\cos{\gamma} + R_x = 0\\
\sum{F_{iy}} = 0 &\Rightarrow  R_y + F_A - W - F_S\sin{\gamma} = 0\\
\sum{M_{i0}} = 0 &\Rightarrow W*b - F_A*(b+d) - F_S\sin{\gamma}*a = 0\\
--&---\\
F_S &= {{W*b - F_A*(b+d)} \over a*\sin{\gamma}}\\
F_S &= {{W*b - F_A*(a+2b+c)} \over a*\sin{\gamma}}\\
--&---\\
R_x &= (-F_S)\cos{\gamma}\\
R_x &= {{F_A*(a+2b+c) - W*b} \over a*\sin{\gamma}})\cos{\gamma}\\
R_x &= {{F_A*(a+2b+c) - W*b} \over a*\sin{\gamma}}\cos{\gamma})\\
R_x &= {{\cot{\gamma} * (F_A*(a+2b+c) - W*b)} \over a}\\
--&---\\
R_y &= W + F_S\sin{\gamma} - F_A\\
R_y &= {{W*b - F_A*(a+2b+c)} \over a*\sin{\gamma}}*\sin{\gamma} + W - F_A\\
R_y &= {{W*(a+b) - F_A*(2(a+b)+c)} \over a}
\end{align}
$$

### Pro B

$$
\begin{align}
\sum{F_{ix}} = 0 &\Rightarrow F_S\cos{\gamma} + R_x = 0\\
\sum{F_{iy}} = 0 &\Rightarrow  R_y + F_B - W - F_S\sin{\gamma} = 0\\
\sum{M_{i0}} = 0 &\Rightarrow W*b + F_B*(a+c) - F_S\sin{\gamma}*a = 0\\
--&---\\
F_S &= {{W*b + F_B*(a+c)} \over a * \sin{\gamma}}\\
--&---\\
R_x &= (-F_S)*\cos{\gamma}\\
R_x &= {{-(W*b + F_B*(a+c))} \over a * \sin{\gamma}}*\cos{\gamma}\\
R_x &= {{-\cot{\gamma}*(W*b + F_B*(a+c))} \over a}\\
--&---\\
R_y &= F_S\sin{\gamma} + W - F_B\\
R_y &= {{W*b + F_B*(a+c)} \over a * \sin{\gamma}}\sin{\gamma} + W - F_B\\
R_y &= {{W*(a+b) + F_B*c} \over a}
\end{align}
$$

### Porovnání

$$
\begin{align}
A_x &\ne B_x\\
{{\cot{\gamma} * (F_A*(a+2b+c) - W*b)} \over a} &\ne {{-\cot{\gamma}*(W*b + F_B*(a+c))} \over a}\\
**&***\\
|\vec{F_A}| = |\vec{F_B}| &\Rightarrow F_A = F \and F_B = F\\
**&***\\
F*(a+2b+c) - W*b &\ne -W*b - F*(a+c))\\
F*(a+b+c) &> 0\\
\bold{A_x} &> \bold{B_x}\\
--&---\\
A_y &\ne B_y\\
{{W*(a+b) - F_A*(2(a+b)+c)} \over a} &\ne {{W*(a+b) + F_B*c} \over a}\\
**&***\\
|\vec{F_A}| = |\vec{F_B}| &\Rightarrow F_A = F \and F_B = F\\
**&***\\
-F*(2(a+b)+c) &\ne F*c\\
F*(a+b+c) &> 0\\
\bold{A_y} &> \bold{B_y}
\end{align}
$$

