$$
\begin{align*}
R_1 &= 99k\Omega\\
R_2 &= 1k\Omega\\
L &= 15.7 mH\\
--&---\\
\hat{P}(j\omega) &= {\hat{U_2} \over \hat{U_1}}\\
\hat{P}(j\omega) &= {{R_2 j \omega L \over R_2+j \omega L}\over {R_1+{R_2 j \omega L \over R_2+j \omega L}}}\\
\hat{P}(j\omega) &= {L R_2 \omega \over -j R_1 R_2 + L R_1 \omega + L R_2 \omega}\\
\hat{P}(j\omega) &= {R_2 \over -{j R_1 R_2 \over L \omega} + R_1 + R_2}\\
\hat{P}(j\omega) &= {R_2 \over R_1 + R_2} {1 \over 1-j{R_1 R_2 \over L \omega (R_1 + R_2)}}\\
\hat{P}(j\omega) &= {R_2 \over R_1 + R_2} {1 \over 1-j\omega{R_1 R_2 \over L \omega^2 (R_1 + R_2)}}\\
\hat{P}(j\omega) &= {R_2 \over R_1 + R_2} {1 \over 1+j{\omega \over \omega_0}}\\
--&---\\
\omega_0 &= -{L\omega^2(R_1+R_2) \over R_1 R_2}\\
\omega_0 &= -{15.7mH\omega^2(99k\Omega+1k\Omega) \over 99k\Omega 1k\Omega}\\
\omega_0 &= -{157 \over 9.9*10^6}\omega^2\\
--&---\\
{R_2 \over R_1 + R_2} &= {1k\Omega \over 99k\Omega+1k\Omega}\\
{R_2 \over R_1 + R_2} &= {1 \over 100}
\end{align*}
$$

![HW03-1](F:\Docs\CTU\b202\ZEO\HW03-1.svg)

![HW03-2](F:\Docs\CTU\b202\ZEO\HW03-2.svg)
